updated and refactored Zulib

src/Zulib/fsharp/Realized/Zen.Types.Realized.fs
@@ -1,0 +1,13 @@
+#light "off"
+module Zen.Types.Realized
+
+type lockCore = {version: uint32; lockData: byte[] list}
+
+
+type contract = {code: byte[]; bounds: byte[]; hint: byte[]}
+
+type extendedContract =
+    | Contract of contract
+    | HighVContract of version : uint32 * data : byte[]
+
+type extraData = byte[] list
