src/Zulib/fstar/Zen.Cost.Extracted.fst
@@ -1,0 +1,104 @@
+module Zen.Cost.Extracted
+
+open Zen.Base
+open Zen.Cost.Realized
+
+val bind2(#a #b #c:Type)(#n1 #n2 #n3:nat):
+  cost a n1 -> cost b n2 -> (a -> b -> cost c n3) -> cost c (n1+n2+n3)
+let bind2 #_ #_ #_ #_ #_ #_ mx my f = mx `bind` (fun x ->
+                                      my `bind` (fun y ->
+                                      f x y))
+
+val bind3(#a #b #c #d:Type)(#n1 #n2 #n3 #n4:nat):
+  cost a n1 -> cost b n2 -> cost c n3 -> (a -> b -> c -> cost d n4)
+  -> cost d (n1+n2+n3+n4)
+let bind3 #_ #_ #_ #_ #_ #_ #_ #_ mx my mz f = mx `bind` (fun x ->
+                                               my `bind` (fun y ->
+                                               mz `bind` (fun z ->
+                                               f x y z)))
+
+val join(#a:Type)(#m #n:nat): cost (cost a n) m -> cost a (n+m)
+let join #_ #_ #_ x =
+  x `bind` (fun z -> z)
+
+val liftM(#a #b:Type)(#n:nat): (a->b) -> cost a n -> cost b n
+let liftM #_ #_ #_ f mx =
+  mx `bind` (f >> ret)
+
+val ap(#a #b:Type)(#m #n:nat): cost (a->b) n -> cost a m -> cost b (n+m)
+let ap #_ #_ #_ #_ mf mx =
+  mf `bind` (fun f -> liftM f mx)
+
+val liftM2(#a #b #c:Type)(#m #n:nat): (a->b->c) -> cost a m -> cost b n
+  -> cost c (m+n)
+let liftM2 #_ #_ #_ #_ #_ f = liftM f >> ap
+
+val liftM3(#a #b #c #d:Type)(#n1 #n2 #n3:nat):
+  (a -> b -> c -> d)
+  -> cost a n1 -> cost b n2 -> cost c n3
+  -> cost d (n1+n2+n3)
+let liftM3 #_ #_ #_ #_ #_ #_ #_ f mx my mz =
+  f `liftM` mx `ap` my `ap` mz
+
+// The "fish". Left to right Kleisli composition of cost.
+val (>=>) (#a #b #c:Type)(#m #n:nat):
+  (a -> cost b n) -> (b -> cost c m) -> (a -> cost c (n+m))
+let (>=>) #_ #_ #_ #_ #_ f g = fun x -> bind (f x) g
+
+// Right to left Kleisli composition of cost.
+val (<=<) (#a #b #c:Type)(#m #n:nat):
+  (b -> cost c n) -> (a -> cost b m) -> (a-> cost c (n+m))
+let (<=<) #_ #_ #_ #_ #_ f g = g >=> f
+
+val eq(#a:eqtype)(#m #n:nat): cost a m -> cost a n -> cost bool (n+m)
+let eq #_ #_ #_ = liftM2 op_Equality
+
+val incRet(#a:Type): n:nat -> a -> cost a n
+let incRet(#_) n x = inc (ret x) n
+
+(** autoInc adds cost to even out branches.*)
+val autoInc(#a:Type)(#m:nat)(#n:nat{m<=n}): cost a m -> cost a n
+let autoInc #_ #m #n mx = inc mx (n-m)
+
+val autoRet(#a:Type)(#m:nat): a -> cost a m
+let autoRet #_ #_ = ret >> autoInc
+
+val retf(#a #b:Type): (a -> b) -> (a -> cost b 0)
+let retf #_ #_ f = f >> ret
+
+//
+// Operators
+//
+unfold let (~!) = ret
+unfold let (+!) k x = inc x k
+unfold let (+~!) = incRet // infix
+unfold let (~+!) = incRet // prefix
+unfold let (>>=) = bind
+unfold let (=<<) f x = bind x f
+unfold let (<$>) = liftM
+unfold let (<$$>) = liftM2
+unfold let (<$$$>) = liftM3
+unfold let (<*>) = ap
+unfold let ( *>) x f = ap f x
+unfold let (<=>) = eq
+unfold let ($>) x f = liftM f x
+val ($$>) (#a #b #c:Type)(#m #n:nat):
+  (cost a m * cost b n) -> (a->b->c) -> cost c (m+n)
+let ($$>) #_ #_ #_ #_ #_ (mx,my) f = liftM2 f mx my
+val ($$$>) (#a #b #c #d:Type)(#n1 #n2 #n3:nat):
+  (cost a n1 * cost b n2 * cost c n3) -> (a->b->c->d) -> cost d (n1+n2+n3)
+let ($$$>) #_ #_ #_ #_ #_ #_ #_ (mx,my,mz) f = liftM3 f mx my mz
+val (<~>) (#a #b:Type)(#n:nat): cost (a->b) n -> a -> cost b n
+let (<~>) #_ #_ #_ mf = ret >> ap mf
+
+// These functions are intentionally not implemented. They cannot be used in actual code.
+// Nevertheless, they are very useful for theorem proving.
+val force_liftM(#a #b:Type)(#n:nat): f:(a -> b) -> mx: cost a n
+  -> Lemma( f (force mx) == force (liftM f mx))
+     [SMTPat (liftM f mx ); SMTPat (f <$> mx); SMTPat (mx $> f)]
+let force_liftM #_ #_ #_ _ _ = ()
+val force_ap: #a:Type -> #b:Type -> #m:nat -> #n:nat
+  -> mf:cost (a -> b) n -> mx: cost a m
+  -> Lemma( (force mf) (force mx) == force (ap mf mx))
+     [SMTPat (ap mf mx); SMTPat (mf <*> mx)]
+let force_ap #_ #_ #_ #_ _ _ = ()
